Change a couple more Definitions to Lemmas proved using exact.

theories/VLSM/Core/Composition.v
@@ -328,20 +328,27 @@ Definition composite_vlsm
   results.
 *)
 Definition composite_apply_plan := (@_apply_plan _ composite_type composite_transition).
-Definition composite_apply_plan_app
+
+Lemma composite_apply_plan_app
   (start : composite_state)
   (a a' : list plan_item)
   : composite_apply_plan start (a ++ a') =
     let (aitems, afinal) := composite_apply_plan start a in
     let (a'items, a'final) := composite_apply_plan afinal a' in
-     (aitems ++ a'items, a'final)
-  := (@_apply_plan_app _ composite_type composite_transition start a a').
-Definition composite_apply_plan_last
+     (aitems ++ a'items, a'final).
+Proof.
+  exact (@_apply_plan_app _ composite_type composite_transition start a a').
+Qed.
+
+Lemma composite_apply_plan_last
   (start : composite_state)
   (a : list plan_item)
   (after_a := composite_apply_plan start a)
-  : finite_trace_last start (fst after_a) = snd after_a
-  := (@_apply_plan_last _ composite_type composite_transition start a).
+  : finite_trace_last start (fst after_a) = snd after_a.
+Proof.
+  exact (@_apply_plan_last _ composite_type composite_transition start a).
+Qed.
+
 Definition composite_trace_to_plan := (@_trace_to_plan _ composite_type).
 
 Lemma composite_initial_state_prop_lift
@@ -395,8 +402,14 @@ Definition lift_to_composite_finite_trace j
   : list (transition_item (IM j)) -> list composite_transition_item
   := VLSM_embedding_finite_trace_project (lift_to_composite_VLSM_embedding j).
 
-Definition lift_to_composite_finite_trace_last j
-  := VLSM_embedding_finite_trace_last (lift_to_composite_VLSM_embedding j).
+Lemma lift_to_composite_finite_trace_last :
+  forall (j : index) (sX : state (IM j)) (trX : list transition_item),
+    lift_to_composite_state' j (finite_trace_last sX trX) =
+    finite_trace_last (lift_to_composite_state' j sX)
+      (VLSM_embedding_finite_trace_project (lift_to_composite_VLSM_embedding j) trX).
+Proof.
+  exact (fun j => VLSM_embedding_finite_trace_last (lift_to_composite_VLSM_embedding j)).
+Qed.
 
 Lemma constraint_free_incl
   (constraint : composite_label -> composite_state  * option message -> Prop)
